F/F_soundness.v
@@ -1,0 +1,627 @@
+Add LoadPath "metatheory".
+Require Export F_init.
+
+Ltac gather_atoms ::=
+  let A := gather_atoms_with (fun x : vars => x) in
+  let B := gather_atoms_with (fun x : var => {{ x }}) in
+  let C := gather_atoms_with (fun x : typing_env => dom x) in
+  let D1 := gather_atoms_with (fun x => fv_term x) in
+  let D2 := gather_atoms_with (fun x => ftv_typ x) in
+  let D3 := gather_atoms_with (fun x => ftv_term x) in
+  constr:(A \u B \u C \u D1 \u D2 \u D3).
+
+(* Mutual induction principles *)
+Scheme pval_mut_ind_aux := Induction for pval Sort Prop
+with   val_mut_ind_aux  := Induction for val  Sort Prop.
+Combined Scheme pval_val_mut_ind from pval_mut_ind_aux, val_mut_ind_aux.
+
+Scheme wfenv_mut_ind_aux := Induction for wfenv Sort Prop
+with   wftyp_mut_ind_aux := Induction for wftyp Sort Prop.
+Combined Scheme wfenv_wftyp_mut_ind from
+  wfenv_mut_ind_aux, wftyp_mut_ind_aux.
+
+(* Administrative lemmas *)
+Lemma var_subst : forall e x, subst_term e x (term_var_f x) = e.
+Proof.
+intros e x; simpl; destruct (x == x); congruence.
+Qed.
+Hint Rewrite var_subst : lngen.
+
+Lemma pval_val_regular :
+  (forall p, pval p → lc_term p) ∧ (forall v, val v → lc_term v).
+Proof.
+apply pval_val_mut_ind; eauto.
+Qed.
+
+Lemma pval_regular : forall p, pval p → lc_term p.
+Proof.
+intros; destruct pval_val_regular as [H1 _]; auto.
+Qed.
+
+Lemma val_regular : forall v, val v → lc_term v.
+Proof.
+intros; destruct pval_val_regular as [_ H2]; auto.
+Qed.
+Hint Resolve pval_regular val_regular.
+
+Lemma red0_regular1 : forall e e', red0 e e' → lc_term e.
+Proof.
+intros e e' H. destruct H; auto.
+Qed.
+
+Lemma red0_regular2 : forall e e', red0 e e' → lc_term e'.
+Proof.
+intros e e' H; destruct H; eauto with lngen.
+Qed.
+Hint Resolve red0_regular1 red0_regular2.
+
+Lemma red1_regular1 : forall e e', e ⇝ e' → lc_term e.
+Proof.
+intros e e' H. induction H; eauto.
+Qed.
+
+Lemma red1_regular2 : forall e e', e ⇝ e' → lc_term e'.
+Proof.
+intros e e' H; induction H; eauto.
+Qed.
+Hint Resolve red1_regular1 red1_regular2.
+
+Lemma wftyp_regular : forall Γ τ, wftyp Γ τ → lc_typ τ.
+Proof.
+intros Γ τ H.
+induction H; eauto.
+Qed.
+Hint Resolve wftyp_regular.
+
+Lemma wfenv_wftyp_aux :
+  (forall Γ, wfenv Γ → forall Γ₁ x τ, Γ = x ~ (Some τ) ++ Γ₁ → wftyp Γ₁ τ) ∧
+  (forall Γ τ, wftyp Γ τ → wfenv Γ).
+Proof.
+apply wfenv_wftyp_mut_ind; intros; eauto.
+inversion H.
+inversion H0; subst; auto.
+inversion H0.
+pick fresh a; assert (a ~ None ++ G ⊢ ok) by auto; inversion H0; subst; auto.
+Qed.
+
+Lemma wfenv_wftyp :
+forall Γ₁ Γ₂ x τ, wfenv (Γ₁ ++ x ~ Some τ ++ Γ₂) → wftyp Γ₂ τ.
+Proof.
+destruct wfenv_wftyp_aux as [H1 H2].
+intros Γ₁ Γ₂ x τ H0.
+generalize dependent Γ₂.
+induction Γ₁; intros; simpl_env in H0; eauto.
+inversion H0; subst; simpl_env in H5; eauto.
+Qed.
+Hint Resolve wfenv_wftyp.
+
+Lemma wftyp_wfenv : forall Γ τ, wftyp Γ τ → wfenv Γ.
+Proof.
+destruct wfenv_wftyp_aux; auto.
+Qed.
+Hint Resolve wftyp_wfenv.
+
+Lemma wfenv_wftyp_uniq_aux :
+  (forall Γ, wfenv Γ → uniq Γ) ∧ (forall Γ τ, wftyp Γ τ → uniq Γ).
+Proof.
+apply wfenv_wftyp_mut_ind; intros; auto.
+pick fresh a. assert (uniq (a ~ None ++ G)) by auto. destruct_uniq; auto.
+Qed.
+
+Lemma wfenv_uniq : forall Γ, wfenv Γ → uniq Γ.
+Proof.
+destruct wfenv_wftyp_uniq_aux; auto.
+Qed.
+Hint Resolve wfenv_uniq.
+
+Lemma wftyp_uniq :  forall Γ τ, wftyp Γ τ → uniq Γ.
+Proof.
+eauto.
+Qed.
+Hint Resolve wftyp_uniq.
+
+Lemma wfenv_wftyp_weakening :
+(forall Γ, wfenv Γ → forall Γ₁ Γ₂ Γ₃, Γ = Γ₁ ++ Γ₃ → wfenv (Γ₂ ++ Γ₃) → disjoint Γ₁ Γ₂ → wfenv (Γ₁ ++ Γ₂ ++ Γ₃))
+∧
+(forall Γ τ, wftyp Γ τ → forall Γ₁ Γ₂ Γ₃, Γ = Γ₁ ++ Γ₃ → wfenv (Γ₂ ++ Γ₃) → disjoint Γ₁ Γ₂ → wftyp (Γ₁ ++ Γ₂ ++ Γ₃) τ).
+Proof.
+apply wfenv_wftyp_mut_ind; intros; auto.
+Case "wfenv_empty".
+destruct Γ₁. destruct Γ₃. simpl_env in *; auto.
+simpl in H; inversion H.
+simpl in H; inversion H.
+Case "wfenv_cons_x".
+destruct Γ₁; simpl_env in *.
+destruct Γ₃; simpl_env in *; auto.
+inversion H0; subst.
+apply wfenv_cons_x.
+simpl in H2; apply disjoint_cons_1 in H2; auto.
+apply H; auto.
+simpl in H2; apply disjoint_cons_2 in H2; auto.
+Case "wfenv_cons_a".
+destruct Γ₁; simpl_env in *.
+destruct Γ₃; simpl_env in *; auto.
+inversion H0; subst.
+apply wfenv_cons_a.
+simpl in H2; apply disjoint_cons_1 in H2; auto.
+apply H; auto.
+simpl in H2; apply disjoint_cons_2 in H2; auto.
+Case "wftyp_var".
+subst G; analyze_binds b.
+Case "wftyp_forall".
+subst G; apply wftyp_forall with (L := L ∪ dom Γ₂); intros.
+rewrite_env ((a~None ++ Γ₁) ++ Γ₂ ++ Γ₃); apply H; eauto.
+Qed.
+
+Lemma wfenv_weakening :
+forall Γ₁ Γ₂ Γ₃, wfenv (Γ₁ ++ Γ₃) → wfenv (Γ₂ ++ Γ₃) → disjoint Γ₁ Γ₂ → wfenv (Γ₁ ++ Γ₂ ++ Γ₃).
+Proof.
+destruct wfenv_wftyp_weakening as [H1 H2].
+intros; apply (H1 (Γ₁ ++ Γ₃)); auto.
+Qed.
+
+Lemma wftyp_weakening :
+forall Γ₁ Γ₂ Γ₃ τ, wftyp (Γ₁ ++ Γ₃) τ → wfenv (Γ₂ ++ Γ₃) → disjoint Γ₁ Γ₂ → wftyp (Γ₁ ++ Γ₂ ++ Γ₃) τ.
+Proof.
+destruct wfenv_wftyp_weakening as [H1 H2].
+intros. apply (H2 (Γ₁ ++ Γ₃)); auto.
+Qed.
+
+Lemma wfenv_wftyp2 :
+forall Γ x τ, wfenv Γ → binds x (Some τ) Γ → wftyp Γ τ.
+Proof.
+intro Γ; induction Γ; intros.
+analyze_binds H0.
+destruct a; destruct o; simpl_env in *; analyze_binds H0.
+replace t with τ in * by congruence.
+rewrite_env (nil ++ a ~ Some τ ++ Γ).
+inversion H; subst.
+apply wftyp_weakening; auto.
+rewrite_env (nil ++ a ~ Some t ++ Γ).
+apply wftyp_weakening; auto. simpl.
+inversion H; subst. eapply IHΓ; eauto.
+rewrite_env (nil ++ a ~ None ++ Γ).
+apply wftyp_weakening; auto.
+inversion H; subst. eapply IHΓ; eauto.
+Qed.
+Hint Resolve wfenv_wftyp2.
+
+Lemma wfenv_regular :
+forall Γ x τ, wfenv Γ → binds x (Some τ) Γ → lc_typ τ.
+Proof.
+intros. induction H; analyze_binds H0.
+replace t with τ in * by congruence; eauto.
+eauto.
+Qed.
+Hint Resolve wfenv_regular.
+
+Lemma wfenv_wftyp_subst :
+  (forall Γ, wfenv Γ → forall Γ₁ Γ₂ x τ, Γ = Γ₁ ++ x ~ (Some τ) ++ Γ₂ → wfenv (Γ₁ ++ Γ₂)) ∧
+  (forall Γ τ, wftyp Γ τ → forall Γ₁ Γ₂ x τ', Γ = Γ₁ ++ x ~ (Some τ') ++ Γ₂ → wftyp (Γ₁ ++ Γ₂) τ).
+Proof.
+apply wfenv_wftyp_mut_ind; intros.
+Case "wfenv_empty".
+assert (binds x (Some τ) nil). rewrite H; auto. analyze_binds H0.
+Case "wfenv_cons_x".
+destruct Γ₁; simpl_env in *.
+inversion H0; subst; eauto.
+destruct p; destruct o; inversion H0; subst; simpl_env in *.
+constructor; eauto.
+Case "wfenv_cons_a".
+destruct Γ₁; simpl_env in *.
+inversion H0; subst; eauto.
+destruct p; destruct o; inversion H0; subst; simpl_env in *.
+constructor; eauto.
+Case "wftyp_var".
+subst G. constructor. analyze_binds b. eauto.
+Case "wftyp_arrow".
+subst G. constructor; eauto.
+Case "wftyp_forall".
+subst G. econstructor; intros.
+rewrite_env (([(a, None)] ++ Γ₁) ++ Γ₂). eapply H; simpl_env; eauto.
+Qed.
+
+Lemma wfenv_subst :
+forall Γ₁ Γ₂ x τ, wfenv (Γ₁ ++ x ~ (Some τ) ++ Γ₂) → wfenv (Γ₁ ++ Γ₂).
+Proof.
+destruct wfenv_wftyp_subst as [H1 H2].
+intros Γ₁ Γ₂ x τ H. eapply H1; eauto.
+Qed.
+Hint Resolve wfenv_subst.
+
+Lemma wftyp_subst :
+forall Γ₁ Γ₂ τ x τ', wftyp (Γ₁ ++ x ~ (Some τ') ++ Γ₂) τ → wftyp (Γ₁ ++ Γ₂) τ.
+Proof.
+destruct wfenv_wftyp_subst as [H1 H2].
+intros. eapply H2; eauto.
+Qed.
+Hint Resolve wftyp_subst.
+
+Lemma wfenv_wftyp_tsubst :
+  (forall Γ, wfenv Γ → forall Γ₁ Γ₂ a τ, Γ = Γ₁ ++ a ~ None ++ Γ₂ → wftyp Γ₂ τ → wfenv ((env_map (tsubst_typ τ a) Γ₁) ++ Γ₂)) ∧
+  (forall Γ τ, wftyp Γ τ → forall Γ₁ Γ₂ a τ', Γ = Γ₁ ++ a ~ None ++ Γ₂ → wftyp Γ₂ τ' → wftyp ((env_map (tsubst_typ τ' a) Γ₁) ++ Γ₂) (tsubst_typ τ' a τ)).
+Proof.
+apply wfenv_wftyp_mut_ind; intros.
+Case "wfenv_empty".
+assert (binds a (@None typ) nil). rewrite H; auto. analyze_binds H1.
+Case "wfenv_cons_x".
+destruct Γ₁; simpl_env in *.
+inversion H0; subst; eauto.
+destruct p; destruct o; inversion H0; subst; simpl_env in *.
+simpl; simpl_env.
+constructor. unfold env_map; auto. eapply H; auto.
+Case "wfenv_cons_a".
+destruct Γ₁; simpl_env in *.
+inversion H0; subst; eauto.
+destruct p; destruct o; inversion H0; subst; simpl_env in *.
+simpl; simpl_env.
+constructor. unfold env_map; auto. eapply H; auto.
+Case "wftyp_var".
+subst G. simpl.
+destruct (a == a0); subst.
+rewrite_env (nil ++ env_map (tsubst_typ τ' a0) Γ₁ ++ Γ₂); apply wftyp_weakening; auto.
+constructor; auto.
+analyze_binds b;
+replace (@None typ) with (option_map (tsubst_typ τ' a0) None) by reflexivity;
+unfold env_map; auto.
+Case "wftyp_arrow".
+subst G. simpl; constructor; auto.
+Case "wftyp_forall".
+subst G. simpl; apply wftyp_forall with (L := L ∪ {{a}}); intros.
+rewrite_env (([(a0, None)] ++ env_map (tsubst_typ τ' a) Γ₁) ++ Γ₂).
+replace ([(a0, None)] ++ env_map (tsubst_typ τ' a) Γ₁) with (env_map (tsubst_typ τ' a) ([(a0, None)] ++ Γ₁)) by reflexivity.
+replace (typ_var_f a0) with (tsubst_typ τ' a (typ_var_f a0)).
+rewrite <- tsubst_typ_open_typ_wrt_typ.
+eapply H; simpl_env; eauto. eauto.
+autorewrite with lngen; auto.
+Qed.
+
+Lemma wfenv_tsubst :
+  forall Γ₁ Γ₂ a τ, wfenv (Γ₁ ++ a ~ None ++ Γ₂) → wftyp Γ₂ τ →
+    wfenv (env_map (tsubst_typ τ a) Γ₁ ++ Γ₂).
+Proof.
+destruct wfenv_wftyp_tsubst as [H1 H2].
+intros Γ₁ Γ₂ x τ H. eapply H1; eauto.
+Qed.
+Hint Resolve wfenv_tsubst.
+
+Lemma wftyp_tsubst :
+forall Γ₁ Γ₂ τ a τ', wftyp (Γ₁ ++ a ~ None ++ Γ₂) τ →
+wftyp Γ₂ τ' → wftyp (env_map (tsubst_typ τ' a) Γ₁ ++ Γ₂) (tsubst_typ τ' a τ).
+Proof.
+destruct wfenv_wftyp_tsubst as [H1 H2].
+intros. eapply H2; eauto.
+Qed.
+Hint Resolve wftyp_tsubst.
+
+Lemma wftyp_fv : forall Γ τ, wftyp Γ τ → ftv_typ τ [<=] dom Γ.
+Proof.
+intros Γ τ H. induction H; simpl in *; try fsetdec.
+assert (a ∈ dom G) by eauto; fsetdec.
+pick fresh a.
+assert (ftv_typ (open_typ_wrt_typ t (typ_var_f a))[<=]add a (dom G)) by auto.
+assert (ftv_typ t [<=] ftv_typ (open_typ_wrt_typ t (typ_var_f a))); auto with lngen.
+fsetdec.
+Qed.
+Hint Resolve wftyp_fv.
+
+Lemma wfterm_wfenv : forall Γ e τ,
+  wfterm Γ e τ → wfenv Γ.
+Proof.
+intros Γ e τ H.
+induction H; auto.
+pick fresh x; assert (wfenv ([(x, Some t1)] ++ G)) by auto; inversion H1; subst; eauto.
+pick fresh a; assert (wfenv ([(a, None)] ++ G)) by auto; inversion H1; subst; eauto.
+Qed.
+Hint Resolve wfterm_wfenv.
+
+Lemma wfterm_wftyp : forall Γ e τ,
+  wfterm Γ e τ → wftyp Γ τ.
+Proof.
+intros Γ e τ H.
+induction H.
+Case "var". eapply wfenv_wftyp2; eauto.
+Case "app". inversion IHwfterm1; subst; auto.
+Case "abs". pick fresh x. assert ([(x, Some t1)] ++ G ⊢ t2 ok) by auto.
+assert (wfenv ([(x, Some t1)] ++ G)) by eauto.
+inversion H2; subst.
+constructor; auto. rewrite_env (nil ++ G). eauto.
+Case "inst". inversion IHwfterm; subst.
+inversion IHwfterm; subst.
+pick fresh a. rewrite tsubst_typ_intro with (a1 := a); auto.
+rewrite_env (env_map (tsubst_typ t a) nil ++ G).
+apply wftyp_tsubst; simpl_env; auto.
+Case "gen".
+apply wftyp_forall with (L := L); auto.
+Qed.
+Hint Resolve wfterm_wftyp.
+
+Lemma wfterm_regular2 : forall Γ e τ,
+  wfterm Γ e τ → lc_typ τ.
+Proof.
+intros Γ e τ H; induction H; eauto.
+Qed.
+Hint Resolve wfterm_regular2.
+
+Lemma wfterm_regular1 : forall Γ e τ,
+  wfterm Γ e τ → lc_term e.
+Proof.
+intros Γ e τ H; induction H; eauto.
+pick fresh x.
+apply lc_term_abs_exists with (x1 := x).
+apply wfenv_regular with (Γ := [(x, Some t1)] ++ G) (x := x); eauto.
+auto.
+Qed.
+Hint Resolve wfterm_regular1.
+
+Lemma wfterm_env_uniq : forall Γ e τ,
+  wfterm Γ e τ → uniq Γ.
+Proof.
+intros Γ e τ H. eauto.
+Qed.
+Hint Resolve wfterm_env_uniq.
+
+(* Lemmas about values *)
+Lemma value_is_normal_aux :
+  (forall v, pval v → ~ exists e, v ⇝ e) ∧
+  (forall v, val v → ~ exists e, v ⇝ e).
+Proof.
+apply pval_val_mut_ind; intros; intros [e0 Hred]; inversion Hred; subst; eauto.
+inversion H.
+inversion H1; subst. inversion p.
+inversion H0; subst. inversion p.
+inversion H0.
+pick fresh x. eapply H; eauto.
+inversion H0.
+pick fresh a. eapply H; eauto.
+Qed.
+
+Lemma value_is_normal : forall v, val v → ~ exists e, v ⇝ e.
+Proof.
+destruct value_is_normal_aux as [_ Th]. intuition auto.
+Qed.
+
+(* Renaming lemmas *)
+Lemma pval_val_renaming : forall x y,
+  (forall v, pval v → pval (subst_term (term_var_f y) x v)) ∧
+  (forall v, val v → val (subst_term (term_var_f y) x v)).
+Proof.
+intros x y.
+apply pval_val_mut_ind; intros; simpl; auto.
+Case "var". destruct (x0 == x); auto.
+Case "abs". pick fresh z and apply val_abs; auto.
+  rewrite subst_term_open_term_wrt_term_var; auto.
+Case "gen". pick fresh a and apply val_gen; auto.
+  rewrite subst_term_open_term_wrt_typ_var; auto.
+Qed.
+
+Lemma val_renaming : forall x y v,
+  val v → val (subst_term (term_var_f y) x v).
+Proof.
+intros x y v H. destruct (pval_val_renaming x y); auto.
+Qed.
+Hint Resolve val_renaming.
+
+(* Lemmas about red0, red1 *)
+Lemma red0_subst : forall x e'' e e', lc_term e'' → red0 e e' →
+  red0 (subst_term e'' x e) (subst_term e'' x e').
+Proof.
+intros x e'' e e' Hlc H.
+inversion H; subst; simpl.
+rewrite subst_term_open_term_wrt_term; auto. apply red0_beta; auto with lngen.
+assert (lc_term (subst_term e'' x (term_abs t e1))) by auto with lngen; auto.
+rewrite subst_term_open_term_wrt_typ; auto. apply red0_beta_t; auto with lngen.
+assert (lc_term (subst_term e'' x (term_gen e0))) by auto with lngen; auto.
+Qed.
+Hint Resolve red0_subst.
+
+Lemma red1_subst : forall x e'' e e', lc_term e'' → e ⇝ e' →
+  (subst_term e'' x e) ⇝ (subst_term e'' x e').
+Proof.
+intros x e'' e e' Hlc H.
+induction H; subst; simpl; auto.
+apply red1_appL; auto with lngen.
+apply red1_appR; auto with lngen.
+apply red1_abs with (L := L `union` {{x}}); auto; intros z Hz.
+replace (term_var_f z) with (subst_term e'' x (term_var_f z)) by auto with lngen.
+repeat rewrite <- subst_term_open_term_wrt_term; eauto.
+apply red1_gen with (L := L `union` {{x}}); intros a Ha.
+repeat rewrite <- subst_term_open_term_wrt_typ; eauto.
+Qed.
+Hint Resolve red1_subst.
+
+Lemma red1_open : forall L e'' e e',
+  lc_term e'' →
+  (forall x, x ∉ L → e ^ x ⇝ e' ^ x) →
+  e ^^ e'' ⇝ e' ^^ e''.
+Proof.
+intros L e'' e e' Hlc H.
+pick fresh x.
+rewrite subst_term_intro with (x1 := x) (e1 := e); auto.
+rewrite subst_term_intro with (x1 := x) (e1 := e'); auto.
+Qed.
+Hint Resolve red1_open.
+
+(*
+(* Lemmas about wfterm *)
+Lemma wfterm_fv : forall Γ e τ,
+  wfterm Γ e τ → fv_term e [<=] dom Γ.
+Proof.
+intros Γ e τ H. induction H; simpl fv_term in *.
+assert (x ∈ dom G) by eauto; fsetdec.
+fsetdec.
+pick fresh x. assert (fv_term (e ^ x) [<=] dom (x ~ t1 ++ G)) by auto.
+assert (fv_term e [<=] fv_term (e ^ x)) by auto with lngen.
+assert (fv_term e [<=] {{x}} ∪ dom G). simpl in *; fsetdec.
+fsetdec.
+Qed.
+
+Lemma wfterm_uniqueness : forall Γ e τ τ',
+  wfterm Γ e τ → wfterm Γ e τ' → τ = τ'.
+Proof.
+intros Γ e τ τ' H1 H2. generalize dependent τ'.
+induction H1; intros τ' H2; inversion H2; subst.
+eauto using binds_unique.
+assert (typ_arrow t2 t1 = typ_arrow t3 τ') by auto; congruence.
+pick fresh x; assert (t2 = t3) by eauto; congruence.
+Qed.
+
+Lemma wfterm_strengthening : forall Γ₁ Γ₂ x τ τ' e,
+  x ∉ fv_term e →
+  wfterm (Γ₁ ++ x ~ τ' ++ Γ₂) e τ →
+  wfterm (Γ₁ ++ Γ₂) e τ.
+Proof.
+intros Γ₁ Γ₂ x τ τ' e Hx He.
+dependent induction He; simpl in Hx.
+Case "var".
+constructor. solve_uniq. analyze_binds_uniq H0.
+Case "app".
+econstructor; eauto.
+Case "abs".
+apply wfterm_abs with (L := L `union` {{x}}); intros.
+rewrite_env (([(x0, t1)] ++ Γ₁) ++ Γ₂).
+eapply H0 with (x1 := x); auto.
+assert (fv_term (e ^ x0) [<=] fv_term (term_var_f x0) ∪ fv_term e) as H2
+ by auto with lngen.
+simpl in H2; fsetdec.
+simpl_env; eauto.
+Qed.
+*)
+
+Lemma wfterm_weakening : forall Γ₁ Γ₂ Γ₃ e τ,
+  wfterm (Γ₁ ++ Γ₃) e τ →
+  wfenv (Γ₂ ++ Γ₃) →
+  disjoint Γ₁ Γ₂ →
+  wfterm (Γ₁ ++ Γ₂ ++ Γ₃) e τ.
+Proof.
+intros Γ₁ Γ₂ Γ₃ e τ H. dependent induction H; intros; eauto.
+Case "var".
+constructor. auto using wfenv_weakening. analyze_binds H0.
+Case "abs". pick fresh x and apply wfterm_abs.
+rewrite_env (([(x, Some t1)] ++ Γ₁) ++ Γ₂ ++ Γ₃).
+apply H0; simpl_env; auto.
+Case "inst". constructor. auto using wftyp_weakening. eauto.
+Case "gen". pick fresh a and apply wfterm_gen.
+rewrite_env (([(a, None)] ++ Γ₁) ++ Γ₂ ++ Γ₃).
+apply H0; simpl_env; auto.
+Qed.
+
+Lemma wfterm_subst : forall Γ₁ Γ₂ x τ₁ τ₂ e₁ e₂,
+  wfterm (Γ₁ ++ x ~ Some τ₂ ++ Γ₂) e₁ τ₁ →
+  wfterm Γ₂ e₂ τ₂ →
+  wfterm (Γ₁ ++ Γ₂) (subst_term e₂ x e₁) τ₁.
+Proof with eauto.
+intros Γ₁ Γ₂ x τ₁ τ₂ e₁ e₂ H. dependent induction H; intro; simpl...
+Case "var".
+  destruct (x == x0); subst.
+  SCase "x = x0".
+    analyze_binds_uniq H0; apply wfterm_weakening with (Γ₁ := nil); auto.
+    replace t with τ₂ by congruence; auto.
+    eapply wfenv_subst; eauto.
+  SCase "x <> x0".
+    analyze_binds_uniq H0...
+Case "abs".
+  pick fresh z and apply wfterm_abs.
+  rewrite_env ((z ~ Some t1 ++ Γ₁) ++ Γ₂).
+  rewrite subst_term_open_term_wrt_term_var...
+  apply H0 with (τ₂0 := τ₂)...
+Case "gen".
+  pick fresh a and apply wfterm_gen.
+  rewrite_env ((a ~ None ++ Γ₁) ++ Γ₂).
+  rewrite subst_term_open_term_wrt_typ_var...
+  apply H0 with (τ₂0 := τ₂)...
+Qed.
+
+Lemma wfterm_tsubst : forall Γ₁ Γ₂ a τ₁ e₁ τ₂,
+  wfterm (Γ₁ ++ a ~ None ++ Γ₂) e₁ τ₁ →
+  wftyp Γ₂ τ₂ →
+  wfterm (env_map (tsubst_typ τ₂ a) Γ₁ ++ Γ₂) (tsubst_term τ₂ a e₁) (tsubst_typ τ₂ a τ₁).
+Proof with eauto.
+intros Γ₁ Γ₂ a τ₁ e₁ τ₂ H. dependent induction H; intro; simpl...
+Case "var".
+constructor. auto using wfenv_tsubst.
+replace (Some (tsubst_typ τ₂ a t)) with (option_map (tsubst_typ τ₂ a) (Some t)) by reflexivity.
+unfold env_map. analyze_binds H0.
+simpl.
+assert (a ∉ ftv_typ t).
+  assert (ftv_typ t [<=] dom Γ₂) by eauto.
+  assert (uniq (Γ₁ ++ [(a, None)] ++ Γ₂)) by auto.
+  destruct_uniq. fsetdec.
+autorewrite with lngen; auto.
+Case "app".
+econstructor.
+eapply IHwfterm1; auto.
+eapply IHwfterm2; auto.
+Case "abs".
+  pick fresh z and apply wfterm_abs.
+  rewrite_env (env_map (tsubst_typ τ₂ a) ([(z, Some t1)] ++ Γ₁) ++ Γ₂).
+  rewrite tsubst_term_open_term_wrt_term_var...
+Case "inst".
+  rewrite tsubst_typ_open_typ_wrt_typ...
+  constructor; auto. apply IHwfterm; auto.
+Case "gen".
+  pick fresh b and apply wfterm_gen.
+  rewrite_env (env_map (tsubst_typ τ₂ a) ([(b, None)] ++ Γ₁) ++ Γ₂).
+  rewrite tsubst_term_open_term_wrt_typ_var...
+  rewrite tsubst_typ_open_typ_wrt_typ_var...
+Qed.
+
+Theorem subject_reduction : forall Γ e e' τ,
+  wfterm Γ e τ → e ⇝ e' → wfterm Γ e' τ.
+Proof with eauto.
+  intros Γ e e' τ H. generalize dependent e'.
+  dependent induction H.
+  Case "var".
+    intros e' J; inversion J; subst; inversion H1.
+  Case "app".
+    intros e' J; inversion J; subst...
+    inversion H; subst; inversion H1; subst.
+    pick fresh z.
+    rewrite (subst_term_intro z)...
+    eapply wfterm_subst with (Γ₁ := nil); simpl_env...
+  Case "abs".
+    intros e' J; inversion J; subst.
+    inversion H1.
+    pick fresh z and apply wfterm_abs...
+  Case "inst".
+    intros e' J; inversion J; subst; auto.
+    inversion H1; subst.
+    inversion H0; subst.
+    pick fresh a.
+    rewrite (tsubst_term_intro a)...
+    rewrite (tsubst_typ_intro a)...
+    rewrite_env (env_map (tsubst_typ t a) nil ++ G).
+    eapply wfterm_tsubst; simpl_env...
+  Case "gen".
+    intros e' J; inversion J; subst.
+    inversion H1.
+    pick fresh a and apply wfterm_gen...
+Qed.
+
+Theorem progress : forall Γ e τ,
+  wfterm Γ e τ →
+  (exists e', e ⇝ e') ∨ val e.
+Proof with eauto 7.
+  intros Γ e τ H.
+  dependent induction H; simpl...
+  Case "typing_app".
+    destruct IHwfterm1 as [[e1' ?] | ?]...
+    destruct IHwfterm2 as [[e2' ?] | ?]...
+    destruct e1; simpl in H1; inversion H1; subst...
+    inversion H.
+  Case "abs".
+    pick fresh z. edestruct (H0 z) as [[e1 ?] | ?]...
+    left.
+      exists (term_abs t1 (close_term_wrt_term z e1)).
+      apply red1_abs with (L := L `union` {{z}}); intros.
+      assert (wfenv ([(z, Some t1)] ++ G)) by eauto.
+      eapply wfenv_regular; eauto.
+      rewrite <- subst_term_spec.
+
+      ICI
+
+      rewrite (subst_term_intro z)...
+    right.
+      apply val_abs with (L := L `union` {{z}}); intros...
+      rewrite (subst_term_intro z)...
+Qed.
